Added arm_rulesTheory - this provides a bunch of theorems of the form:
X => (NEXT_ARMe s = s')

where "s" is the state and "X" provides a context i.e. the instruction (at the
program counter address) and any constraints on the register arguments.  This
will be progressively expanded (as needed) to cover more of the instruction
space.

examples/arm6/evaluate/arm_evalScript.sml
@@ -41,12 +41,12 @@ val SET_BYTE_def = Define`
       (24 <= i /\ i < 32) /\ (if oareg = 3w then b %% (i - 24) else x)) w`;
 
 val MEM_WRITE_BYTE_def = Define`
-  MEM_WRITE_BYTE (mem:mem) (word:word32) addr =
+  MEM_WRITE_BYTE (mem:mem) addr (word:word32) =
     let addr30 = ADDR30 addr in
       (addr30 :- SET_BYTE ((1 >< 0) addr) ((7 >< 0) word) (mem addr30)) mem`;
 
 val MEM_WRITE_WORD_def = Define`
-  MEM_WRITE_WORD (mem:mem) word addr = (ADDR30 addr :- word) mem`;
+  MEM_WRITE_WORD (mem:mem) addr word = (ADDR30 addr :- word) mem`;
 
 val MEM_WRITE_def = Define`
   MEM_WRITE b = if b then MEM_WRITE_BYTE else MEM_WRITE_WORD`;
@@ -56,7 +56,7 @@ val TRANSFERS_def = Define`
   (TRANSFERS mem data (r::rs) =
    case r of
       MemRead addr -> TRANSFERS mem (SNOC (mem (ADDR30 addr)) data) rs
-   || MemWrite b addr word -> TRANSFERS (MEM_WRITE b mem word addr) data rs
+   || MemWrite b addr word -> TRANSFERS (MEM_WRITE b mem addr word) data rs
    || _ -> TRANSFERS mem data rs)`;
 
 val NEXT_ARMe_def = Define`
